examples/iterators/Dup_Utils.dfy
@@ -31,9 +31,9 @@ lemma DupDupRev<A>(xs: seq<A>)
        Dup(xs);
        [xs[0]] + [xs[0]] + Dup(xs[1..]);
        [xs[0]] + [xs[0]] + DupRev(xs[1..]);
-       {assert |xs[1..]|==|xs|-1 >=1; 
-       assert xs[1..][|xs|-2]== xs[|xs|-1];
-       assert xs[1..][..|xs|-2]== xs[1..|xs|-1];}
+       {assert |xs[1..]| == |xs|-1 >=1; 
+       assert xs[1..][|xs|-2] == xs[|xs|-1];
+       assert xs[1..][..|xs|-2] == xs[1..|xs|-1];}
        [xs[0]] + [xs[0]]  + (DupRev(xs[1..|xs|-1]) + [xs[|xs|-1]] + [xs[|xs|-1]]);
        DupRev(xs[..|xs|-1]) + [xs[|xs|-1]] + [xs[|xs|-1]];
        DupRev(xs);
@@ -46,17 +46,17 @@ lemma DupDupRev<A>(xs: seq<A>)
 
 lemma {:induction xs} SetDup<A>(xs: seq<A>)
 ensures forall x :: x in xs <==> x in Dup(xs)
-ensures |Dup(xs)|==2*|xs|
-ensures forall i | 0<=i<|xs| :: xs[i]==Dup(xs)[2*i]==Dup(xs)[2*i+1]
+ensures |Dup(xs)| == 2*|xs|
+ensures forall i | 0 <= i < |xs| :: xs[i] == Dup(xs)[2*i] == Dup(xs)[2*i+1]
 {}
 
  lemma {:induction xs} DupElsAux<A>(xs: seq<A>,x:A)
  requires x in xs
- ensures multiset(Dup(xs))[x]==2*multiset(xs)[x]
+ ensures multiset(Dup(xs))[x] == 2*multiset(xs)[x]
 {
-    if (xs==[]){}
+    if (xs == []){}
     else{
-      if (x==xs[0]){
+      if (x == xs[0]){
           if (xs[0] in xs[1..]){
             calc=={
               multiset(Dup(xs))[xs[0]];
@@ -74,8 +74,8 @@ ensures forall i | 0<=i<|xs| :: xs[i]==Dup(xs)[2*i]==Dup(xs)[2*i+1]
               {SetDup(xs[1..]);
               assert xs[0] !in xs[1..] ==> xs[0] !in Dup(xs[1..]);
               assert multiset(Dup(xs[1..]))[xs[0]]==0;}
-              2;{assert xs==[xs[0]]+xs[1..];
-                assert multiset(xs)[xs[0]]==1;}
+              2;{assert xs == [xs[0]]+xs[1..];
+                assert multiset(xs)[xs[0]] == 1;}
               2*multiset(xs)[xs[0]];
             }
       }
@@ -84,7 +84,7 @@ ensures forall i | 0<=i<|xs| :: xs[i]==Dup(xs)[2*i]==Dup(xs)[2*i+1]
         calc=={
          multiset(Dup(xs))[x];
          multiset(Dup(xs[1..]))[x];{assert x in xs[1..];}
-         2*multiset(xs[1..])[x];{assert xs==[xs[0]]+xs[1..];}
+         2*multiset(xs[1..])[x];{assert xs == [xs[0]]+xs[1..];}
          2*multiset(xs)[x];
        }
 
@@ -98,9 +98,9 @@ ensures forall i | 0<=i<|xs| :: xs[i]==Dup(xs)[2*i]==Dup(xs)[2*i+1]
 
 
 lemma {:induction xs} DupEls<A>(xs: seq<A>)
- ensures forall x | x in xs :: multiset(Dup(xs))[x]==2*multiset(xs)[x]
+ ensures forall x | x in xs :: multiset(Dup(xs))[x] == 2*multiset(xs)[x]
 { forall x | x in xs 
-  ensures multiset(Dup(xs))[x]==2*multiset(xs)[x]{
+  ensures multiset(Dup(xs))[x] == 2*multiset(xs)[x]{
    DupElsAux(xs,x);
 
   }
@@ -108,9 +108,9 @@ lemma {:induction xs} DupEls<A>(xs: seq<A>)
 
 
 function DupI(i:int,j:int):int
-ensures i==j==> DupI(i,j)==2*i
-ensures i!=j ==> DupI(i,j)==2*i+1
-{if (i==j) then 2*i
+ensures i == j ==> DupI(i,j) == 2*i
+ensures i != j ==> DupI(i,j) == 2*i+1
+{if (i == j) then 2*i
  else 2*i+1}
  
 
@@ -119,8 +119,8 @@ function DupF(j:int):(int -> int)
 
 
 function DupInvariant(i:int,j:int):int
-ensures i<j==> DupInvariant(i,j)==2*i+1
-ensures i>=j ==> DupInvariant(i,j)==j+i
+ensures i < j  ==> DupInvariant(i,j) == 2*i+1
+ensures i >= j ==> DupInvariant(i,j) == j+i
 {if (i < j) then 2*i+1
  else i+j}
 
@@ -129,4 +129,4 @@ function DupInvariantF(j:int):(int -> int)
 { i => DupInvariant(i,j) }
 
 function DupMapI<A>(xs:seq<A>,i:int):map<int,int>
-{(map it | -1<=it<=|xs| :: if (it < i) then 2*it+1 else i+it)}
+{(map it | -1 <= it <= |xs| :: if (it < i) then 2*it+1 else i+it)}
